ulib/FStar.Tactics.Builtins.fst
@@ -147,22 +147,32 @@ with all this. *)
 assume val t_exact : bool -> bool -> term -> Tac unit
 
 (** Inner primitive for [apply], takes a boolean specifying whether
-to not ask for implicits that appear free in posterior goals. Example:
-when the boolean is true, applying transitivity to
-[|- a = c] will give two goals, [|- a = ?u] and [|- ?u = c] without
-asking to instantiate [?u] since it will most likely be constrained
-later by solving these goals. In any case, we track [?u] and will fail
-if it's not solved later.
+to not ask for implicits that appear free in posterior goals, and a
+boolean specifying whether it's forbidden to instantiate uvars in the
+goal.
 
-You probably want [apply] from FStar.Tactics.Derived.
+Example: when [uopt] is true, applying transitivity to [|- a = c]
+will give two goals, [|- a = ?u] and [|- ?u = c] without asking to
+instantiate [?u] since it will most likely be constrained later by
+solving these goals. In any case, we track [?u] and will fail if it's
+not solved later.
+
+Example: when [noinst] is true, applying a function returning
+[1 = 2] will fail on a goal of the shape [1 = ?u] since it must
+instantiate [?u]. We use this in typeclass resolution.
+
+You may want [apply] from FStar.Tactics.Derived, or one of
+the other user facing variants.
 *)
-assume val t_apply : bool -> bool -> term -> Tac unit
+assume val t_apply : uopt:bool -> noinst:bool -> term -> Tac unit
 
-(** [apply_lemma l] will solve a goal of type [squash phi] when [l] is a Lemma
-ensuring [phi]. The arguments to [l] and its requires clause are introduced as new goals.
-As a small optimization, [unit] arguments are discharged by the engine. *)
+(** [t_apply_lemma l] will solve a goal of type [squash phi] when [l] is
+a Lemma ensuring [phi]. The arguments to [l] and its requires clause are
+introduced as new goals. As a small optimization, [unit] arguments are
+discharged by the engine. For the meanining of the [noinst] boolean arg
+see [t_apply]. *)
+assume val t_apply_lemma : noinst:bool -> term -> Tac unit
 // TODO: do the unit thing too for [apply].
-assume val apply_lemma : term -> Tac unit
 
 (** [print str] has no effect on the proofstate, but will have the side effect
 of printing [str] on the compiler's standard output. *)
